%%%%%%%% this is the Appendix A n in data generation paper
%%%%%%%% details of deriving C_m

%\input{template.tex}
%\begin{document}

In our approach it is very crucial to derive \Cm based on a known $R(P,Q)$, the detailed steps to derive \Cm from model 1 (\ref{model1}) is given below,

%% C_m(P,Q) 
%% C_1\left(C_2 - e^{-a|\phi_P|} - e^{-a|\phi_Q|} + e^{-a|\phi_P - \phi_Q|}\right)

\begin{eqnarray*}
	R(P, Q) &=& R(\phi_P, \phi_Q, \Delta \lambda) = \tilde{C}(\phi_P, \phi_Q) \frac{1-p^2}{1 - 2p \cos(\Theta)+p^2},
\end{eqnarray*}

where $\Theta = \Delta \lambda + u(\phi_P - \phi_Q),$ with some choice of $C_1, C_2, a, u,$ and $p$.

Now,

\begin{eqnarray*}
	C_m(\phi_P, \phi_Q) &=& \frac{1}{2\pi} \int_{-\pi}^\pi R(\phi_P, \phi_Q, \Delta \lambda) e^{-im\Delta \lambda}d\Delta \lambda \\
	&=& \tilde{C}(\phi_P, \phi_Q) \frac{1}{2\pi}\int_{-\pi}^\pi \frac{1-p^2}{1 - 2p \cos(\Theta+p^2} e^{-im\Delta \lambda}d\Delta \lambda
\end{eqnarray*}

Next we focus on the following integration.

\begin{eqnarray*}
	\int_{-\pi}^\pi \frac{1-p^2}{1 - 2p \cos(x+b)+p^2} e^{-imx}dx ,
\end{eqnarray*}

where we set $x=\Delta\lambda$ and $b=u(\phi_P -\phi_Q)$ and we have,

\begin{eqnarray*}
	\frac{1-p^2}{1 - 2p \cos(x+b)+p^2} &=& \frac{2-2p\cos(x+b)-(1-2p \cos(x+b)+p^2)}{1-2p \cos(x+b)+p^2}\\
	&=& 2\times \frac{1-p\cos(x+b)}{1-2p \cos(x+b)+p^2}-1 \\
	&=& 2\times \sum_{n=0}^{\infty}p^n\cos n(x+b)-1  \\
	&=& 1 + 2 \sum_{n=1}^{\infty}p^n (\cos nx \cos(nb) - \sin(nx) \sin(nb)).
\end{eqnarray*}
Therefore, for $m \ne 0$,
\begin{eqnarray*}
	& & \int_{-\pi}^\pi \frac{1-p^2}{1 - 2p \cos(x+b)+p^2} e^{-imx}dx \\
	&=& \int_{-\pi}^\pi \left[1 + 2 \sum_{n=1}^{\infty}p^n (\cos nx \cos(nb) - \sin(nx) \sin(nb))\right]  e^{-imx}dx \\
	&=& \int_{-\pi}^\pi e^{-imx}dx + 2 \sum_{n=1}^{\infty}p^n \int_{-\pi}^\pi \left[\cos nx \cos(nb) - \sin(nx) \sin(nb)\right]  e^{-imx}dx \\
	&=& 2 \sum_{n=1}^{\infty}p^n \left[\cos(nb)  \int_{-\pi}^\pi \cos(nx) e^{-imx} dx - \sin(nb)  \int_{-\pi}^\pi \sin(nx) e^{-imx}dx \right] \\
	&=& 2 \sum_{n=1}^{\infty}p^n \left[ \pi \cos(nb) \delta(n, m) + \pi i\sin(nb)\right] \\
	&=& 2\pi p^m e^{imb}
\end{eqnarray*}
That is, for $m \ne 0$,

\begin{eqnarray*}
	C_m(\phi_P, \phi_Q)  &=& \tilde{C}(\phi_P, \phi_Q) \frac{1}{2\pi} (2\pi p^m e^{imb}) \\
	&=& \tilde{C}(\phi_P, \phi_Q) p^m e^{imb}.
\end{eqnarray*}
And for $m = 0$, $C_0(\phi_P, \phi_Q) = \tilde{C}(\phi_P, \phi_Q)$.\\

In summary,

\begin{eqnarray*}
	C_m(\phi_P, \phi_Q) &=& \left\{ \begin{array}{ll}
	\tilde{C}(\phi_P, \phi_Q), & m = 0 \\
	\tilde{C}(\phi_P, \phi_Q)p^m e^{imb}, & m \ne 0.
	\end{array}
	\right.\\
	%&=& C_1\left(C_2 - e^{-a|\phi_P|} - e^{-a|\phi_Q|} + e^{-a|\phi_P - \phi_Q|}\right)p^m (\cos(mu(\phi_P - \phi_Q))+i \sin(mu(\phi_P - \phi_Q))).
\end{eqnarray*}

If the process is longitudinally reversible one can set $u=0$ suppose $\tilde{C}(\phi_P, \phi_Q)$ given by \ref{Cm_model1} then \Cm for model1,

\begin{eqnarray*}
	C_m(\phi_P, \phi_Q) &=& \left\{ \begin{array}{ll}
	C_1\left(C_2 - e^{-a|\phi_P|} - e^{-a|\phi_Q|} + e^{-a|\phi_P - \phi_Q|}\right)  & m = 0 \\
	C_1\left(C_2 - e^{-a|\phi_P|} - e^{-a|\phi_Q|} + e^{-a|\phi_P - \phi_Q|}\right)p^m & m \ne 0.
	\end{array}
	\right.
\end{eqnarray*}




%\end{document}
